coq/dec/Proof.v
@@ -1,8 +1,122 @@
 Require Import Syntax.
 Require Import Algo.
+Require Import Lia.
+From Hammer Require Import Tactics.
+Require Import Coq.Program.Equality.
 
 (*
 for references of previous systems:
 1. https://types.hk/proof/contextual/README.html
 2. https://github.com/juniorxxue/contextual-typing/blob/main/paper_extended.pdf (Page 32)
 *)
+
+Fixpoint term_size (e : term) : nat :=
+  match e with
+  | Lit _ => 1
+  | Var _ => 1
+  | Lam e' => 1 + term_size e'
+  | App e1 e2 => 2 + term_size e1 + term_size e2
+  | Ann e' _ => 1 + term_size e'
+  | TLam e' => 1 + term_size e'
+  | TApp e' _ => 1 + term_size e'
+  end.
+
+Fixpoint context_size (Σ : context) : nat :=
+  match Σ with
+  | ctxEmpty => 0
+  | ctxType _ => 0
+  | ctxTerm e Σ' => 1 + term_size e + context_size Σ'
+  | ctxTApp _ Σ' => 1 + context_size Σ'
+  end.
+
+Fixpoint type_size (A : type) : nat :=
+  match A with
+  | Int => 1
+  | TVar _ => 1
+  | Arr A1 A2 => 1 + type_size A1 + type_size A2
+  | Fall A' => 1 + type_size A'
+  end.
+
+Lemma dec_NonEmpty Σ :
+  {Σ = ctxEmpty} + {nonEmpty Σ}.
+Proof. sauto lq: on. Qed.
+
+Lemma dec_lookup Γ n :
+  (exists A, lookup Γ n A) \/ ~ (exists A, lookup Γ n A).
+Proof.
+  revert n; induction Γ; intros n.
+  - sauto lq: on.
+  - destruct n.
+    + sauto lq: on.
+    + destruct (IHΓ n) as [[A H] | H]; sauto lq: on.
+  - destruct (IHΓ n) as [[A H] | H]; sauto lq: on.
+Qed.
+
+Lemma lookup_det Γ n A A' :
+  lookup Γ n A -> lookup Γ n A' -> A = A'.
+Proof.
+  revert n A A'; induction Γ; intros n A A' H1 H2; sauto lq: on rew: off.
+Qed.
+
+Lemma dec_ty_sub : forall n,
+  (forall Γ Σ e, term_size e + context_size Σ < n ->
+    (exists A, ty Γ Σ e A) \/ ~ (exists A, ty Γ Σ e A)) /\
+  (forall Γ Σ A, context_size Σ < n ->
+    sub Γ A Σ \/ ~ sub Γ A Σ).
+Proof.
+  intros n. induction n. split; try lia.
+  destruct IHn as [IHty IHsub]. split.
+  - intros Γ Σ e Hlt.
+    destruct e; simpl in *.
+    + destruct (dec_NonEmpty Σ).
+      * sauto lq: on rew: off.
+      * assert (DecSub: sub Γ Int Σ \/ ~ sub Γ Int Σ).
+        { eapply IHsub. lia. }
+        destruct DecSub.
+        -- sauto lq: on.
+        -- right. intros [A Contra].
+           dependent destruction Contra.
+           ++ hauto lq: on.
+           ++ dependent destruction Contra.
+              sfirstorder. sauto lq: on.
+    + destruct (dec_NonEmpty Σ); destruct (dec_lookup Γ n0) as [[A Hlkup] | Hlkup].
+      * sauto lq: on.
+      * right. intros [A Contra].
+        dependent destruction Contra; sauto lq: on.
+      * assert (DecSub: sub Γ A Σ \/ ~ sub Γ A Σ).
+        { eapply IHsub. lia. }
+        destruct DecSub.
+        -- sauto lq: on.
+        -- right. intros [A' Contra].
+          dependent destruction Contra.
+          ++ sauto lq: on use: lookup_det.
+          ++ dependent destruction Contra.
+            ** eapply lookup_det with (A := A0) in Hlkup; eauto.
+               sfirstorder.
+            ** sauto lq: on.
+      * right. intros [A Contra].
+        dependent destruction Contra.
+        -- sfirstorder use: lookup_det.
+        -- dependent destruction Contra; sauto lq: on.
+    + admit.
+    + admit.
+    + admit.
+    + admit.
+    + admit. 
+  - intros Γ Σ A Hlt.
+    destruct Σ; simpl in *.
+    + sfirstorder.
+    + admit.
+    + destruct A.
+      * sauto lq: on.
+      * sauto lq: on.
+      * assert (DecSub: sub Γ A2 Σ \/ ~ sub Γ A2 Σ).
+        { eapply IHsub. lia. }
+        assert (DecTy: (exists C, ty Γ (ctxType A1) t C) \/
+                     ~ (exists C, ty Γ (ctxType A1) t C)).
+        { eapply IHty. simpl. lia. }
+        destruct DecSub; destruct DecTy as [[C Hty] | Hty]; sauto lq: on.
+      * sauto lq: on.
+    + right. intros Contra.
+      dependent destruction Contra.
+Admitted.
